split file into 3

theories/trans_correctness_continuations.v
@@ -2,727 +2,20 @@ Require Import syntax.
 Require Import small_step tactics.
 Require Import sequences.
 Require Import typing.
+Require Import continuations.
 
-Definition process_exceptions := 
-  (Lam (* x => *) (Lam (* y => *) 
-    (Match_ (Var 0 (* y *)) (* with *)
-      (* | None => *)
-        (Var 1 (* y *))
-      (* | Some z => *)
-        (Match_ (Var 2 (* x *)) (* with *)
-          (* | None => *)
-            (Var 1 (* y *))
-          (* | Some w => *)
-            (Conflict)
-        )
-      ))).
-
-
-Fixpoint trans_ty (ty: type): type :=
-  match ty with
-  | TBool => TBool
-  | TInteger => TInteger
-  | TFun T1 T2 => TFun (trans_ty T1) (trans_ty T2)
-  | TOption T => TOption (trans_ty T)
-  | TUnit => TUnit
-  | TDefault T => TOption (trans_ty T)
-  | TArray T => TArray (trans_ty T)
-  end
-.
-
-Fixpoint trans (t: term) : term :=
-  match t with
-  | Var x => Var x
-  | App t1 t2 => App (trans t1) (trans t2)
-  | Lam t => Lam (trans t)
-
-  | Value v => Value (trans_value v)
-  | Binop op t1 t2 => Binop op (trans t1) (trans t2)
-
-  | Match_ u t1 t2 =>
-    Match_ (trans u) (trans t1) (trans t2)
-  | ENone => ENone
-  | ESome t => ESome (trans t)
-
-  | If t ta tb =>
-    If (trans t) (trans ta) (trans tb)
-  | Fold f ts acc =>
-    Fold (trans f) (trans ts) (trans acc)
-
-  | ErrorOnEmpty t => Match_ (trans t) Conflict (Var 0)
-  | DefaultPure t => ESome (trans t)
-  | Default ts tj tc =>
-    Match_
-      (Fold 
-        process_exceptions
-        (EArray (List.map trans ts)) ENone)
-      (If (trans tj) (trans tc) ENone)
-      (ESome (Var 0))
-  | Empty => ENone
-  | Conflict => Conflict
-  | EArray ts => EArray (List.map trans ts)
-  end
-
-with trans_value v :=
-  match v with
-  | Bool b => Bool b
-  | Int i => Int i
-  | Closure t sigma => Closure (trans t) (List.map trans_value sigma)
-  | VNone => VNone
-  | VUnit => VUnit
-  | VSome v => VSome (trans_value v)
-  | VPure v => VSome (trans_value v)
-  | VArray vs => VArray (List.map trans_value vs)
-  end
-.
-
-Inductive no_default: term -> Prop :=
-  | NDVar: forall x, no_default (Var x)
-  | NDApp: forall t1 t2,
-    no_default t1 ->
-    no_default t2 ->
-    no_default (App t1 t2)
-  | NDLam: forall t,
-    no_default t ->
-    no_default (Lam t)
-
-  | NDConflict:
-    no_default Conflict
-
-  | NDValue: forall v,
-    no_default_value v ->
-    no_default (Value v)
-  | NDBinop: forall op t1 t2,
-    no_default t1 ->
-    no_default t2 ->
-    no_default (Binop op t1 t2)
-
-  | NDMatch_: forall u t1 t2,
-    no_default u ->
-    no_default t1 ->
-    no_default t2 ->
-    no_default (Match_ u t1 t2)
-  | NDENone:
-    no_default ENone
-  | NDESome: forall t,
-    no_default t ->
-    no_default (ESome t)
-  | NDFold: forall f ts t,
-    no_default f ->
-    no_default ts ->
-    no_default t ->
-    no_default (Fold f ts t)
-  | NDIf: forall t ta tb,
-    no_default t ->
-    no_default ta ->
-    no_default tb ->
-    no_default (If t ta tb)
-
-  | NDArray: forall ts,
-    List.Forall no_default ts ->
-    no_default (EArray ts)
-
-with no_default_value: value -> Prop :=
-  | NDBool: forall b, no_default_value (Bool b)
-  | NDInt: forall i, no_default_value (Int i)
-  | NDClosure: forall t sigma,
-    no_default t ->
-    List.Forall no_default_value sigma ->
-    no_default_value (Closure t sigma)
-  | NDVNone:
-    no_default_value VNone
-  | NDVUnit:
-    no_default_value VUnit
-  | NDVSome: forall v,
-    no_default_value v ->
-    no_default_value (VSome v)
-  | NDVPure: forall v,
-    no_default_value v ->
-    no_default_value (VPure v)
-  | NDVArray: forall vs,
-    List.Forall no_default_value vs ->
-    no_default_value (VArray vs)
-.
-
-
-
-Theorem no_more_defaults:
-  forall t, no_default (trans t)
-with no_more_defaults_value:
-  forall v, no_default_value (trans_value v).
-Proof.
-{ induction t; simpl; repeat econstructor; eauto.
-  { induction ts; econstructor; eauto. }
-  { induction ts; econstructor; eauto. }
-}
-{ induction v; simpl; repeat econstructor; eauto.
-  { induction sigma; econstructor; eauto. }
-  { induction ts; econstructor; eauto. }
-}
-Qed.
-
-
-Lemma trans_ty_inv_base {T}:
-  inv_base (trans_ty T)
-with trans_ty_inv_no_immediate_default {T}:
-  inv_no_immediate_default (trans_ty T).
-Proof.
-  all: induction T; simpl; econstructor; eauto.
-Qed.
-
-Lemma trans_ty_correct_term:
-  forall {t Delta Gamma T},
-    jt_term Delta Gamma t T ->
-    jt_term Delta (List.map trans_ty Gamma) (trans t) (trans_ty T)
-.
-Proof.
-  intros.
-  apply (
-    jt_term_ind'
-      (fun Delta Gamma t T => jt_term Delta (List.map trans_ty Gamma) (trans t) (trans_ty T))
-      (fun Delta t T => jt_value Delta (trans_value t) (trans_ty T))).
-
-  (* TODO: remove the timeout to put something else. *)
-  all: try solve [timeout 3 (intros; simpl; repeat econs_jt; simpl in *; eauto; repeat econs_inv; eauto using trans_ty_inv_base, trans_ty_inv_no_immediate_default)].
-  { intros; simpl; econstructor.
-    { erewrite List.map_nth_error; eauto. }
-    { eapply trans_ty_inv_base. }
-  }
-  { intros; simpl; repeat econs_jt; simpl in *; eauto using trans_ty_inv_base, trans_ty_inv_no_immediate_default.
-    12:{ clear -f2'. induction f2'; simpl; econstructor; eauto. }
-
-    all: try solve [repeat econs_inv; eauto using trans_ty_inv_base, trans_ty_inv_no_immediate_default].
-  }
-  { intros; simpl; repeat econs_jt; simpl in *; eauto using trans_ty_inv_base, trans_ty_inv_no_immediate_default. 
-    { induction op; simpl in *; inj; eauto. }
-  }
-  { intros; simpl; repeat econs_jt; simpl in *; eauto using trans_ty_inv_base, trans_ty_inv_no_immediate_default.
-    { clear -f8'; induction f8'; simpl; econstructor; eauto. }
-  }
-  { intros; simpl. eapply (JTValueClosure _ _ _ (List.map trans_ty Gamma_cl)); repeat econs_jt; simpl in *; repeat econs_inv; eauto using trans_ty_inv_base, trans_ty_inv_no_immediate_default.
-    { clear - f17'; induction f17'; econstructor; simpl; eauto. }
-    {  repeat sinv_jt; eauto. }
-  }
-  { intros; simpl; repeat econs_jt; simpl in *; eauto using trans_ty_inv_base, trans_ty_inv_no_immediate_default.
-    { clear -f22'; induction f22'; simpl; econstructor; eauto. }
-  }
-Qed.
-
-Lemma trans_ty_correct_value:
-  forall {v Delta T},
-    jt_value Delta v T ->
-    jt_value Delta (trans_value v) (trans_ty T).
-Proof.
-  intros.
-  apply (
-    jt_value_ind'
-      (fun Delta Gamma t T => jt_term Delta (List.map trans_ty Gamma) (trans t) (trans_ty T))
-      (fun Delta t T => jt_value Delta (trans_value t) (trans_ty T))).
-
-  (* TODO: remove the timeout to put something else. *)
-  all: try solve [timeout 3 (intros; simpl; repeat econs_jt; simpl in *; eauto; repeat econs_inv; eauto using trans_ty_inv_base, trans_ty_inv_no_immediate_default)].
-  { intros; simpl; econstructor.
-    { erewrite List.map_nth_error; eauto. }
-    { eapply trans_ty_inv_base. }
-  }
-  { intros; simpl; repeat econs_jt; simpl in *; eauto using trans_ty_inv_base, trans_ty_inv_no_immediate_default.
-    12:{ clear -f2'. induction f2'; simpl; econstructor; eauto. }
-
-    all: try solve [repeat econs_inv; eauto using trans_ty_inv_base, trans_ty_inv_no_immediate_default].
-  }
-  { intros; simpl; repeat econs_jt; simpl in *; eauto using trans_ty_inv_base, trans_ty_inv_no_immediate_default. 
-    { induction op; simpl in *; inj; eauto. }
-  }
-  { intros; simpl; repeat econs_jt; simpl in *; eauto using trans_ty_inv_base, trans_ty_inv_no_immediate_default.
-    { clear -f8'; induction f8'; simpl; econstructor; eauto. }
-  }
-  { intros; simpl. eapply (JTValueClosure _ _ _ (List.map trans_ty Gamma_cl)); repeat econs_jt; simpl in *; repeat econs_inv; eauto using trans_ty_inv_base, trans_ty_inv_no_immediate_default.
-    { clear - f17'; induction f17'; econstructor; simpl; eauto. }
-    {  repeat sinv_jt; eauto. }
-  }
-  { intros; simpl; repeat econs_jt; simpl in *; eauto using trans_ty_inv_base, trans_ty_inv_no_immediate_default.
-    { clear -f22'; induction f22'; simpl; econstructor; eauto. }
-  }
-Qed.
-
-Theorem term_ind' : forall P : term -> Prop,
-  (forall x : var, P (Var x)) ->
-  (forall t1 : term, P t1 -> forall t2 : term, P t2 -> P (App t1 t2)) ->
-  (forall t : {bind term}, P t -> P (Lam t)) ->
-  (forall arg : term, P arg -> P (ErrorOnEmpty arg)) ->
-  (forall arg : term, P arg -> P (DefaultPure arg)) ->
-  forall (IHDef: forall (ts : list term), List.Forall P ts -> forall (tj : term),
-  P tj -> forall tc : term, P tc -> P (Default ts tj tc)),
-  P Empty ->
-  P Conflict ->
-  (forall v : value, P (Value v)) ->
-  (forall (op : op) (t1 : term),
-  P t1 -> forall t2 : term, P t2 -> P (Binop op t1 t2)) ->
-  (forall u : term,
-  P u ->
-  forall t1 : term,
-  P t1 -> forall t2 : {bind term}, P t2 -> P (Match_ u t1 t2)) ->
-  P ENone ->
-  (forall t : term, P t -> P (ESome t)) ->
-  forall (IHFold: forall f : {bind 2 of term},
-  P f -> forall ts, P ts -> forall (t : term), P t -> P (Fold f ts t)),
-  forall IHArray: (forall (ts : list term), List.Forall P ts -> P (EArray ts)),
-  (forall t : term,
-  P t ->
-  forall ta : term, P ta -> forall tb : term, P tb -> P (If t ta tb)) ->
-  forall t : term, P t.
-Proof.
-  intros until t; revert t.
-  fix IHt 1; lock IHt.
-  induction t; eauto.
-  { eapply IHDef; eauto.
-    unlock IHt; clear -IHt.  
-    induction ts; econstructor; eauto.
-  }
-  { eapply IHArray; eauto.
-    unlock IHt; clear -IHt.  
-    induction ts; econstructor; eauto.
-  }
-Qed.
-
-
-Lemma trans_te_renaming:
-  forall t u,
-  trans t = u ->
-  forall xi,
-  trans t.[ren xi] = u.[ren xi].
-Proof.
-  induction t using term_ind'; repeat (asimpl; intros; subst; f_equal; eauto).
-  { induction H; simpl; f_equal; eauto. }
-  { induction H; simpl; f_equal; eauto. }
-Qed.
-
-
-
-Theorem trans_te_substitution_aux:
-  forall t u,
-  trans t = u ->
-  forall sigma1 sigma2,
-  (forall x, trans (sigma1 x) = sigma2 x) ->
-  trans t.[sigma1] = u.[sigma2].
-Proof.
-  induction t using term_ind'; try solve [repeat (asimpl; intros; subst; f_equal; eauto)].
-  { asimpl; intros; subst. asimpl. f_equal.
-    eapply IHt; eauto.
-    { intros. induction x; asimpl; eauto.
-      eapply trans_te_renaming.
-      eauto.
-    }
-  }
-  { repeat (asimpl; intros; subst).
-    repeat f_equal; eauto.
-    induction H; asimpl; eauto; repeat f_equal; eauto.
-  }
-  { intros; subst; asimpl; f_equal; eauto.
-    eapply IHt3; eauto.
-    { intros. induction x; asimpl; eauto.
-      eapply trans_te_renaming.
-      eauto.
-    }
-  }
-  { repeat (asimpl; intros; subst).
-    repeat f_equal; eauto.
-    induction H; asimpl; eauto; repeat f_equal; eauto.
-  }
-Qed.
-
-Theorem trans_te_substitution:
-  forall t,
-  forall sigma1 sigma2,
-  List.Forall2 (fun v1 v2 => trans_value v1 = v2) sigma1 sigma2 ->
-  trans t.[subst_of_env sigma1] = (trans t).[subst_of_env sigma2].
-Proof.
-  intros.
-  eapply trans_te_substitution_aux; eauto.
-  intro a; revert a.
-  induction H, a; asimpl; eauto. rewrite H; eauto.
-Qed. 
+Require Import trans_definition.
 
 Require Import common.
 
-Theorem trans_te_substitution_0:
-  forall t v,
-  trans t.[Value v/] = (trans t).[Value (trans_value v)/].
-Proof.
-  intros.
-  replace (scons (Value v) ids) with (subst_of_env (v::nil)).
-  replace (scons (Value (trans_value v)) ids) with (subst_of_env ((trans_value v)::nil)).
-  eapply trans_te_substitution; eauto.
-
-  
-  { eapply FunctionalExtensionality.functional_extensionality; intros.
-    induction x; unfold subst_of_env; simpl; eauto; rewrite nth_error_nil; f_equal; lia. }
-  { eapply FunctionalExtensionality.functional_extensionality; intros.  
-    induction x; unfold subst_of_env; simpl; eauto; rewrite nth_error_nil; f_equal; lia.
-  }
-Qed.
-
-
-Lemma Forall2_map: forall sigma,
-  List.Forall2 (fun v1 v2 : value => trans_value v1 = v2) sigma
-    (List.map trans_value sigma).
-Proof.
-  induction sigma; econstructor; eauto.
-Qed.
-
-Lemma trans_value_op_correct:
-  forall v op v1 v2,
-    Some v = get_op op v1 v2 ->
-    Some (trans_value v) = get_op op (trans_value v1) (trans_value v2).
-Proof.
-  induction op, v1 , v2; intros; simpl in *; inj; simpl; eauto.
-Qed.
-
 Import List.ListNotations.
 Open Scope list.
-
-
-Lemma array_one_value:
-  forall v,
-  [(Value v)] = (List.map (fun vi => Value vi) [v]).
-Proof.
-  simpl; eauto.
-Qed.
-
-Lemma array_nil_value:
-  [] = (List.map (fun vi => Value vi) []).
-Proof.
-  simpl; eauto.
-Qed.
-
-Lemma cons_is_app [A]:
-  forall (h: A) t,
-  h::t = [h] ++ t.
-Proof.
-  simpl; eauto.
-Qed.
-
-Lemma trans_comm_value:
-  forall v,
-  trans (Value v) = Value (trans_value v).
-Proof.
-  simpl; eauto.
-Qed.
-
-Lemma map_trans_comm_value:
-  forall vs,
-  List.map trans (List.map (fun vi => Value vi) vs)
-  = List.map (fun vi => Value vi) (List.map trans_value vs).
-Proof.
-  induction vs; simpl; eauto.
-  { rewrite IHvs.
-    eauto.
-  }
-Qed.
-
-
-
-Theorem correction_small_steps:
-  forall s1 s2,
-  sred s1 s2 ->
-  exists target,
-    star sred
-      (trans s1) target /\
-    star sred
-      (trans s2) target.
-Proof.
-
-  Local Ltac step := (
-    try (eapply step_left; [solve [repeat econstructor; simpl; eauto; repeat intro; tryfalse]|]);
-    try (eapply step_right; [solve [repeat econstructor; simpl; eauto; repeat intro; tryfalse]|])
-  ).
-
-  intros s1 s2.
-  intros Hsred.
-  induction Hsred; intros; unpack.
-  (* When the right hand side is the result of the left hand side. *)
-  all: try solve [simpl; repeat step; eapply diagram_finish].
-  { asimpl. repeat step. eexists; split; simpl trans; [|eapply star_refl; fail].
-    rewrite <- List.map_cons.
-    eapply star_refl_eq.
-    symmetry.
-    eapply trans_te_substitution; eauto.
-    eapply Forall2_map.
-  }
-  { simpl; repeat step; eexists; split; asimpl; eapply star_trans; eauto with sred; eapply star_refl. }
-  { simpl; repeat step; eexists; split; asimpl; eapply star_trans; eauto with sred; eapply star_refl. }
-  { simpl; repeat step.
-    eapply step_left. { econstructor; simpl; eapply trans_value_op_correct; eauto. }
-    eapply diagram_finish.
-  }
-  { simpl; repeat step; eexists; split; asimpl; eapply star_trans; eauto with sred; eapply star_refl. }
-  { simpl; repeat step; eexists; split; asimpl; eapply star_trans; eauto with sred; eapply star_refl. }
-  { simpl.
-    (* Sadly, direct application of econstructor does not work here. Hence we need to apply the correct steps by hand. *)
-    eapply step_left.
-    { econstructor. econstructor.
-      replace nil with (List.map (fun vi => Value vi) nil) by (simpl; 
-      eauto).
-      econstructor.
-    }
-    eapply step_left.
-    { econstructor.
-      (* econstructor fails here because fold tries first to apply the first argument, whereas it should first apply the second one *)
-      Fail solve [econstructor; eauto].
-
-      eapply sred_Fold_step.
-      econstructor.
-    }
-    eapply step_left.
-    { econstructor.
-      eapply sred_Fold_finish.
-    }
-
-    (* After those manual steps, we finally arrive to the correct term *)
-    eapply step_left; [econstructor|].
-    eapply step_left; [econstructor|].
-    eapply diagram_finish.
-  }
-  { simpl.
-    (* Sadly, direct application of econstructor does not work here. Hence we need to apply the correct steps by hand. *)
-    eapply step_left.
-    { econstructor. econstructor.
-      replace nil with (List.map (fun vi => Value vi) nil) by (simpl; 
-      eauto).
-      econstructor.
-    }
-    eapply step_left.
-    { econstructor.
-      (* econstructor fails here because fold tries first to apply the first argument, whereas it should first apply the second one *)
-      Fail solve [econstructor; eauto].
-
-      eapply sred_Fold_step.
-      econstructor.
-    }
-    eapply step_left.
-    { econstructor.
-      eapply sred_Fold_finish.
-    }
-
-    (* After those manual steps, we finally arrive to the correct term *)
-    eapply step_left; [econstructor|].
-    eapply step_left; [econstructor|].
-    eapply diagram_finish.
-  }
-  { simpl.
-    eapply step_left. {
-      replace nil with (List.map (fun vi => Value vi) nil) by (simpl; eauto).
-      repeat econstructor.
-    }
-    eapply step_left. {
-      econstructor.
-      eapply sred_Fold_step.
-      econstructor.
-    }
-    eapply step_left. {
-      econstructor.
-      eapply sred_Fold_finish.
-    }
-    eapply step_left; [econstructor|].
-    eapply step_left; [econstructor|].
-    eapply diagram_finish.
-  }
-  { simpl.
-    eapply step_left. {
-      replace nil with (List.map (fun vi => Value vi) nil) by (simpl; eauto).
-      repeat econstructor.
-    }
-    eapply step_left. {
-      econstructor.
-      eapply sred_Fold_step.
-      econstructor.
-    }
-    eapply step_left. {
-      econstructor.
-      eapply sred_Fold_finish.
-    }
-    eapply step_right. {
-      replace nil with (List.map (fun vi => Value vi) nil) by (simpl; eauto).
-      repeat econstructor.
-    }
-    eapply step_right. {
-      econstructor.
-      eapply sred_Fold_step.
-      econstructor.
-    }
-    eapply step_right. {
-      econstructor.
-      eapply sred_Fold_finish.
-    }
-    eapply step_left; [econstructor|].
-    eapply step_right; [econstructor|].
-    eapply star_step_left; [eapply star_sred_if_cond; eauto|].
-    eapply star_step_right; [eapply star_sred_if_cond; eauto|].
-    eapply diagram_finish.
-  }
-  { simpl.
-    (* need termination for this proof. *)
-    admit.
-  }
-  { simpl.
-    eapply step_left. {
-      rewrite array_one_value.
-      repeat econstructor.
-    }
-    eapply step_left. {
-      econstructor.
-      eapply sred_Fold_step.
-      econstructor.
-    }
-    eapply step_left. {
-      econstructor.
-      eapply sred_Fold_rec.
-    }
-    eapply step_left. { econstructor; eapply sred_Fold_step; repeat econstructor. }
-    eapply step_left. { econstructor; eapply sred_Fold_step; repeat econstructor. }
-    eapply step_left. { econstructor; eapply sred_Fold_step; repeat econstructor. }
-    eapply step_left. { econstructor; eapply sred_Fold_step; repeat econstructor. }
-    eapply step_left. { econstructor; eapply sred_Fold_step; repeat econstructor. }
-    simpl.
-    eapply step_left. { econstructor; eapply sred_Fold_finish; repeat econstructor. }
-    eapply step_left. { repeat econstructor. }
-    simpl.
-    eapply step_left. { repeat econstructor. }
-    eapply diagram_finish.
-  }
-  { simpl.
-    eapply step_left. {
-      econstructor.
-      eapply sred_Fold_args.
-      rewrite <- (List.app_nil_l (Conflict :: List.map trans ts2)).
-      rewrite array_nil_value.
-      eapply sred_array_conflict.
-    }
-    eapply step_left. {
-      econstructor.
-      eapply sred_Fold_args_Conflict.
-    }
-    eapply step_left; [econstructor|].
-    eapply diagram_finish.
-  }
-
-  { simpl.
-    eapply step_left. {
-      econstructor.
-      eapply sred_Fold_args.
-      rewrite cons_is_app.
-      rewrite array_one_value.
-      eapply sred_array_conflict.
-    }
-    eapply step_left. {
-      econstructor.
-      eapply sred_Fold_args_Conflict.
-    }
-    eapply step_left; [econstructor|].
-    eapply diagram_finish.
-  }
-  { simpl.
-    admit "need terminaison".
-  }
-  { simpl.
-    admit "need terminaison".
-  }
-  { simpl.
-    eapply star_step_left. {
-      eapply star_sred_match_cond.
-      eapply star_sred_fold_args.
-      rewrite cons_is_app.
-      rewrite array_one_value.
-      eapply star_sred_array_ctx.
-      eauto.
-    }
-    eapply star_step_right. {
-      eapply star_sred_match_cond.
-      eapply star_sred_fold_args.
-      rewrite cons_is_app.
-      rewrite array_one_value.
-      eapply star_sred_array_ctx.
-      eauto.
-    }
-    eapply diagram_finish.
-  }
-  { simpl.
-    eapply star_step_left. {
-      eapply star_sred_match_cond.
-      eapply star_sred_fold_args.
-      rewrite <- (List.app_nil_l (trans ti :: List.map trans ts2)).
-      rewrite array_nil_value.
-      eapply star_sred_array_ctx.
-      eauto.
-    }
-    eapply star_step_right. {
-      eapply star_sred_match_cond.
-      eapply star_sred_fold_args.
-      rewrite <- (List.app_nil_l (trans ti' :: List.map trans ts2)).
-      rewrite array_nil_value.
-      eapply star_sred_array_ctx.
-      eauto.
-    }
-    eapply diagram_finish.
-  }
-  { simpl; repeat step. eexists; split; asimpl; eapply star_refl_eq; eauto.
-    eapply trans_te_substitution_0. }
-  { simpl; repeat step; eexists; split; asimpl; eapply star_trans; eauto with sred; eapply star_refl. }
-  { simpl; repeat step; eexists; split; asimpl; eapply star_trans; eauto with sred; eapply star_refl. }
-  { simpl; repeat step; eexists; split; asimpl; eapply star_trans; eauto with sred; eapply star_refl. }
-  { simpl; repeat step; eexists; split; asimpl; eapply star_trans; eauto with sred; eapply star_refl. }
-  { simpl; repeat step; eexists; split; asimpl; eapply star_trans; eauto with sred; eapply star_refl. }
-  { simpl.
-    eapply star_step_left. { eapply star_sred_fold_args; eauto. }
-    eapply star_step_right. { eapply star_sred_fold_args; eauto. }
-    eapply diagram_finish.
-  }
-  { simpl.
-    eapply star_step_left. { eapply star_sred_fold; eauto. }
-    eapply star_step_right. { eapply star_sred_fold; eauto. }
-    eapply diagram_finish.
-  }
-  { simpl.
-    eapply star_step_left. {
-      rewrite List.map_app.
-      rewrite List.map_cons.
-      rewrite map_trans_comm_value.
-      eapply star_sred_array_ctx; eauto.
-    }
-    eapply star_step_right. {
-      rewrite List.map_app.
-      rewrite List.map_cons.
-      rewrite map_trans_comm_value.
-      eapply star_sred_array_ctx; eauto.
-    }
-    eapply diagram_finish.
-  }
-  { simpl.
-    eapply step_left. {
-      rewrite List.map_app.
-      rewrite List.map_cons.
-      rewrite map_trans_comm_value.
-      simpl.
-      eapply sred_array_conflict; eauto.
-    }
-    eapply diagram_finish.
-  }
-  { simpl.
-    eapply step_left. {
-      rewrite map_trans_comm_value.
-      econstructor.
-    }
-    eapply diagram_finish.
-  }
-Admitted.
-
 
 (** Translation correctness using continuations. *)
 
 
 (* To prove the translation correctness using continuations, we first need to extend the trans statement to states. This require to expand the definition to `cont`, `state`, `return` as well to `environements`. *)
 
-Require Import continuations.
 
 
 
@@ -897,6 +190,9 @@ Proof.
   }
 Qed.
 
+
+(** Auxiliary lemmas about the derivations *)
+
 Lemma CArray2_reduces:
   forall t ts vs1 vs2 sigma,
   forall Delta Gamma T,
@@ -1015,7 +311,7 @@ Proof.
   { right. eauto. }
 Qed.
 
-Local Ltac step' := (
+Local Ltac step := (
   (* This tatic try to advance the computation on the right or on the left of the diagram. *)
   try (eapply step_left; [solve
     (* generic case *)
@@ -1124,7 +420,7 @@ Proof.
   induction 1; intros.
   all: induction o; unfold process_exceptions in *; repeat (sinv_jt; inj; subst; simpl in *; subst).
   all: fold process_exceptions in *.
-  all: repeat step'.
+  all: repeat step.
   all: try solve [
     eapply diagram_finish | eapply IHFilteredForall2; repeat econs_jt; eauto
   ].
@@ -1253,16 +549,16 @@ Proof.
 
   all:
     try solve [
-      repeat step';
+      repeat step;
       try eapply diagram_finish;
       eauto
     ].
 
   all: learn (trans_ty_state_correct Hjt).
 
-  { simpl. repeat step'.
+  { simpl. repeat step.
     induction ts.
-    { repeat step'; eapply diagram_finish. }
+    { repeat step; eapply diagram_finish. }
     { clear IHts. intros.
       eapply step_left; [econstructor|].
       eapply step_right; [econstructor|].
@@ -1325,7 +621,7 @@ Proof.
       eapply diagram_finish.
     }
   }
-  { simpl. repeat step'.
+  { simpl. repeat step.
 
     repeat sinv_jt.
     assert (Hjt1:
@@ -1383,7 +679,7 @@ Proof.
     }
     eapply diagram_finish.
   }
-  { simpl. repeat step'.
+  { simpl. repeat step.
     (* same *)
 
     repeat sinv_jt.
@@ -1441,10 +737,10 @@ Proof.
     }
     eapply diagram_finish.
   }
-  { simpl; repeat step'.
+  { simpl; repeat step.
     induction ts; simpl.
-    { repeat step'; eapply diagram_finish. }
-    { repeat step'.
+    { repeat step; eapply diagram_finish. }
+    { repeat step.
       (* same *)
 
       repeat sinv_jt.
@@ -1505,10 +801,10 @@ Proof.
       eapply diagram_finish.
     }
   }
-  { simpl; repeat step'.
+  { simpl; repeat step.
     induction ts; simpl.
-    { repeat step'. eapply diagram_finish. }
-    { clear IHts. repeat step'.
+    { repeat step. eapply diagram_finish. }
+    { clear IHts. repeat step.
       (* require an variant of the previous mentionned lemma to inducate we will go into a fatal error. *)
 
       repeat sinv_jt.
@@ -1548,14 +844,14 @@ Proof.
       { erewrite append_stack_2; [simpl with_stack|simpl; eauto].
         eapply star_cred_append_stack; eauto.
       }
-      repeat step'.
+      repeat step.
       eapply diagram_finish.
     }
   }
   (* Only two cases are left. *)
   { tryfalse. }
   { (* require list rewriting. *)
-    simpl; repeat step'; simpl.
+    simpl; repeat step; simpl.
     rewrite List.map_app, List.map_rev; simpl.
     eapply diagram_finish.
   }
