theories/trans_correctness_small_steps.v
@@ -1,0 +1,469 @@
+Require Import syntax.
+Require Import small_step tactics.
+Require Import sequences.
+Require Import typing.
+
+Require Import trans_definition.
+
+Import List.ListNotations.
+Open Scope list.
+
+
+Theorem term_ind' : forall P : term -> Prop,
+  (forall x : var, P (Var x)) ->
+  (forall t1 : term, P t1 -> forall t2 : term, P t2 -> P (App t1 t2)) ->
+  (forall t : {bind term}, P t -> P (Lam t)) ->
+  (forall arg : term, P arg -> P (ErrorOnEmpty arg)) ->
+  (forall arg : term, P arg -> P (DefaultPure arg)) ->
+  forall (IHDef: forall (ts : list term), List.Forall P ts -> forall (tj : term),
+  P tj -> forall tc : term, P tc -> P (Default ts tj tc)),
+  P Empty ->
+  P Conflict ->
+  (forall v : value, P (Value v)) ->
+  (forall (op : op) (t1 : term),
+  P t1 -> forall t2 : term, P t2 -> P (Binop op t1 t2)) ->
+  (forall u : term,
+  P u ->
+  forall t1 : term,
+  P t1 -> forall t2 : {bind term}, P t2 -> P (Match_ u t1 t2)) ->
+  P ENone ->
+  (forall t : term, P t -> P (ESome t)) ->
+  forall (IHFold: forall f : {bind 2 of term},
+  P f -> forall ts, P ts -> forall (t : term), P t -> P (Fold f ts t)),
+  forall IHArray: (forall (ts : list term), List.Forall P ts -> P (EArray ts)),
+  (forall t : term,
+  P t ->
+  forall ta : term, P ta -> forall tb : term, P tb -> P (If t ta tb)) ->
+  forall t : term, P t.
+Proof.
+  intros until t; revert t.
+  fix IHt 1; lock IHt.
+  induction t; eauto.
+  { eapply IHDef; eauto.
+    unlock IHt; clear -IHt.  
+    induction ts; econstructor; eauto.
+  }
+  { eapply IHArray; eauto.
+    unlock IHt; clear -IHt.  
+    induction ts; econstructor; eauto.
+  }
+Qed.
+
+
+Lemma trans_te_renaming:
+  forall t u,
+  trans t = u ->
+  forall xi,
+  trans t.[ren xi] = u.[ren xi].
+Proof.
+  induction t using term_ind'; repeat (asimpl; intros; subst; f_equal; eauto).
+  { induction H; simpl; f_equal; eauto. }
+  { induction H; simpl; f_equal; eauto. }
+Qed.
+
+
+
+Theorem trans_te_substitution_aux:
+  forall t u,
+  trans t = u ->
+  forall sigma1 sigma2,
+  (forall x, trans (sigma1 x) = sigma2 x) ->
+  trans t.[sigma1] = u.[sigma2].
+Proof.
+  induction t using term_ind'; try solve [repeat (asimpl; intros; subst; f_equal; eauto)].
+  { asimpl; intros; subst. asimpl. f_equal.
+    eapply IHt; eauto.
+    { intros. induction x; asimpl; eauto.
+      eapply trans_te_renaming.
+      eauto.
+    }
+  }
+  { repeat (asimpl; intros; subst).
+    repeat f_equal; eauto.
+    induction H; asimpl; eauto; repeat f_equal; eauto.
+  }
+  { intros; subst; asimpl; f_equal; eauto.
+    eapply IHt3; eauto.
+    { intros. induction x; asimpl; eauto.
+      eapply trans_te_renaming.
+      eauto.
+    }
+  }
+  { repeat (asimpl; intros; subst).
+    repeat f_equal; eauto.
+    induction H; asimpl; eauto; repeat f_equal; eauto.
+  }
+Qed.
+
+Theorem trans_te_substitution:
+  forall t,
+  forall sigma1 sigma2,
+  List.Forall2 (fun v1 v2 => trans_value v1 = v2) sigma1 sigma2 ->
+  trans t.[subst_of_env sigma1] = (trans t).[subst_of_env sigma2].
+Proof.
+  intros.
+  eapply trans_te_substitution_aux; eauto.
+  intro a; revert a.
+  induction H, a; asimpl; eauto. rewrite H; eauto.
+Qed. 
+
+Require Import common.
+
+Theorem trans_te_substitution_0:
+  forall t v,
+  trans t.[Value v/] = (trans t).[Value (trans_value v)/].
+Proof.
+  intros.
+  replace (scons (Value v) ids) with (subst_of_env (v::nil)).
+  replace (scons (Value (trans_value v)) ids) with (subst_of_env ((trans_value v)::nil)).
+  eapply trans_te_substitution; eauto.
+
+  
+  { eapply FunctionalExtensionality.functional_extensionality; intros.
+    induction x; unfold subst_of_env; simpl; eauto; rewrite nth_error_nil; f_equal; lia. }
+  { eapply FunctionalExtensionality.functional_extensionality; intros.  
+    induction x; unfold subst_of_env; simpl; eauto; rewrite nth_error_nil; f_equal; lia.
+  }
+Qed.
+
+
+Lemma Forall2_map: forall sigma,
+  List.Forall2 (fun v1 v2 : value => trans_value v1 = v2) sigma
+    (List.map trans_value sigma).
+Proof.
+  induction sigma; econstructor; eauto.
+Qed.
+
+Lemma array_one_value:
+  forall v,
+  [(Value v)] = (List.map (fun vi => Value vi) [v]).
+Proof.
+  simpl; eauto.
+Qed.
+
+Lemma array_nil_value:
+  [] = (List.map (fun vi => Value vi) []).
+Proof.
+  simpl; eauto.
+Qed.
+
+Lemma cons_is_app [A]:
+  forall (h: A) t,
+  h::t = [h] ++ t.
+Proof.
+  simpl; eauto.
+Qed.
+
+Lemma trans_comm_value:
+  forall v,
+  trans (Value v) = Value (trans_value v).
+Proof.
+  simpl; eauto.
+Qed.
+
+Lemma map_trans_comm_value:
+  forall vs,
+  List.map trans (List.map (fun vi => Value vi) vs)
+  = List.map (fun vi => Value vi) (List.map trans_value vs).
+Proof.
+  induction vs; simpl; eauto.
+  { rewrite IHvs.
+    eauto.
+  }
+Qed.
+
+
+
+Theorem correction_small_steps:
+  forall s1 s2,
+  sred s1 s2 ->
+  exists target,
+    star sred
+      (trans s1) target /\
+    star sred
+      (trans s2) target.
+Proof.
+
+  Local Ltac step := (
+    try (eapply step_left; [solve [repeat econstructor; simpl; eauto; repeat intro; tryfalse]|]);
+    try (eapply step_right; [solve [repeat econstructor; simpl; eauto; repeat intro; tryfalse]|])
+  ).
+
+  intros s1 s2.
+  intros Hsred.
+  induction Hsred; intros; unpack.
+  (* When the right hand side is the result of the left hand side. *)
+  all: try solve [simpl; repeat step; eapply diagram_finish].
+  { asimpl. repeat step. eexists; split; simpl trans; [|eapply star_refl; fail].
+    rewrite <- List.map_cons.
+    eapply star_refl_eq.
+    symmetry.
+    eapply trans_te_substitution; eauto.
+    eapply Forall2_map.
+  }
+  { simpl; repeat step; eexists; split; asimpl; eapply star_trans; eauto with sred; eapply star_refl. }
+  { simpl; repeat step; eexists; split; asimpl; eapply star_trans; eauto with sred; eapply star_refl. }
+  { simpl; repeat step.
+    eapply step_left. { econstructor; simpl; eapply trans_value_op_correct; eauto. }
+    eapply diagram_finish.
+  }
+  { simpl; repeat step; eexists; split; asimpl; eapply star_trans; eauto with sred; eapply star_refl. }
+  { simpl; repeat step; eexists; split; asimpl; eapply star_trans; eauto with sred; eapply star_refl. }
+  { simpl.
+    (* Sadly, direct application of econstructor does not work here. Hence we need to apply the correct steps by hand. *)
+    eapply step_left.
+    { econstructor. econstructor.
+      replace nil with (List.map (fun vi => Value vi) nil) by (simpl; 
+      eauto).
+      econstructor.
+    }
+    eapply step_left.
+    { econstructor.
+      (* econstructor fails here because fold tries first to apply the first argument, whereas it should first apply the second one *)
+      Fail solve [econstructor; eauto].
+
+      eapply sred_Fold_step.
+      econstructor.
+    }
+    eapply step_left.
+    { econstructor.
+      eapply sred_Fold_finish.
+    }
+
+    (* After those manual steps, we finally arrive to the correct term *)
+    eapply step_left; [econstructor|].
+    eapply step_left; [econstructor|].
+    eapply diagram_finish.
+  }
+  { simpl.
+    (* Sadly, direct application of econstructor does not work here. Hence we need to apply the correct steps by hand. *)
+    eapply step_left.
+    { econstructor. econstructor.
+      replace nil with (List.map (fun vi => Value vi) nil) by (simpl; 
+      eauto).
+      econstructor.
+    }
+    eapply step_left.
+    { econstructor.
+      (* econstructor fails here because fold tries first to apply the first argument, whereas it should first apply the second one *)
+      Fail solve [econstructor; eauto].
+
+      eapply sred_Fold_step.
+      econstructor.
+    }
+    eapply step_left.
+    { econstructor.
+      eapply sred_Fold_finish.
+    }
+
+    (* After those manual steps, we finally arrive to the correct term *)
+    eapply step_left; [econstructor|].
+    eapply step_left; [econstructor|].
+    eapply diagram_finish.
+  }
+  { simpl.
+    eapply step_left. {
+      replace nil with (List.map (fun vi => Value vi) nil) by (simpl; eauto).
+      repeat econstructor.
+    }
+    eapply step_left. {
+      econstructor.
+      eapply sred_Fold_step.
+      econstructor.
+    }
+    eapply step_left. {
+      econstructor.
+      eapply sred_Fold_finish.
+    }
+    eapply step_left; [econstructor|].
+    eapply step_left; [econstructor|].
+    eapply diagram_finish.
+  }
+  { simpl.
+    eapply step_left. {
+      replace nil with (List.map (fun vi => Value vi) nil) by (simpl; eauto).
+      repeat econstructor.
+    }
+    eapply step_left. {
+      econstructor.
+      eapply sred_Fold_step.
+      econstructor.
+    }
+    eapply step_left. {
+      econstructor.
+      eapply sred_Fold_finish.
+    }
+    eapply step_right. {
+      replace nil with (List.map (fun vi => Value vi) nil) by (simpl; eauto).
+      repeat econstructor.
+    }
+    eapply step_right. {
+      econstructor.
+      eapply sred_Fold_step.
+      econstructor.
+    }
+    eapply step_right. {
+      econstructor.
+      eapply sred_Fold_finish.
+    }
+    eapply step_left; [econstructor|].
+    eapply step_right; [econstructor|].
+    eapply star_step_left; [eapply star_sred_if_cond; eauto|].
+    eapply star_step_right; [eapply star_sred_if_cond; eauto|].
+    eapply diagram_finish.
+  }
+  { simpl.
+    (* need termination for this proof. *)
+    admit.
+  }
+  { simpl.
+    eapply step_left. {
+      rewrite array_one_value.
+      repeat econstructor.
+    }
+    eapply step_left. {
+      econstructor.
+      eapply sred_Fold_step.
+      econstructor.
+    }
+    eapply step_left. {
+      econstructor.
+      eapply sred_Fold_rec.
+    }
+    eapply step_left. { econstructor; eapply sred_Fold_step; repeat econstructor. }
+    eapply step_left. { econstructor; eapply sred_Fold_step; repeat econstructor. }
+    eapply step_left. { econstructor; eapply sred_Fold_step; repeat econstructor. }
+    eapply step_left. { econstructor; eapply sred_Fold_step; repeat econstructor. }
+    eapply step_left. { econstructor; eapply sred_Fold_step; repeat econstructor. }
+    simpl.
+    eapply step_left. { econstructor; eapply sred_Fold_finish; repeat econstructor. }
+    eapply step_left. { repeat econstructor. }
+    simpl.
+    eapply step_left. { repeat econstructor. }
+    eapply diagram_finish.
+  }
+  { simpl.
+    eapply step_left. {
+      econstructor.
+      eapply sred_Fold_args.
+      rewrite <- (List.app_nil_l (Conflict :: List.map trans ts2)).
+      rewrite array_nil_value.
+      eapply sred_array_conflict.
+    }
+    eapply step_left. {
+      econstructor.
+      eapply sred_Fold_args_Conflict.
+    }
+    eapply step_left; [econstructor|].
+    eapply diagram_finish.
+  }
+
+  { simpl.
+    eapply step_left. {
+      econstructor.
+      eapply sred_Fold_args.
+      rewrite cons_is_app.
+      rewrite array_one_value.
+      eapply sred_array_conflict.
+    }
+    eapply step_left. {
+      econstructor.
+      eapply sred_Fold_args_Conflict.
+    }
+    eapply step_left; [econstructor|].
+    eapply diagram_finish.
+  }
+  { simpl.
+    admit "need terminaison".
+  }
+  { simpl.
+    admit "need terminaison".
+  }
+  { simpl.
+    eapply star_step_left. {
+      eapply star_sred_match_cond.
+      eapply star_sred_fold_args.
+      rewrite cons_is_app.
+      rewrite array_one_value.
+      eapply star_sred_array_ctx.
+      eauto.
+    }
+    eapply star_step_right. {
+      eapply star_sred_match_cond.
+      eapply star_sred_fold_args.
+      rewrite cons_is_app.
+      rewrite array_one_value.
+      eapply star_sred_array_ctx.
+      eauto.
+    }
+    eapply diagram_finish.
+  }
+  { simpl.
+    eapply star_step_left. {
+      eapply star_sred_match_cond.
+      eapply star_sred_fold_args.
+      rewrite <- (List.app_nil_l (trans ti :: List.map trans ts2)).
+      rewrite array_nil_value.
+      eapply star_sred_array_ctx.
+      eauto.
+    }
+    eapply star_step_right. {
+      eapply star_sred_match_cond.
+      eapply star_sred_fold_args.
+      rewrite <- (List.app_nil_l (trans ti' :: List.map trans ts2)).
+      rewrite array_nil_value.
+      eapply star_sred_array_ctx.
+      eauto.
+    }
+    eapply diagram_finish.
+  }
+  { simpl; repeat step. eexists; split; asimpl; eapply star_refl_eq; eauto.
+    eapply trans_te_substitution_0. }
+  { simpl; repeat step; eexists; split; asimpl; eapply star_trans; eauto with sred; eapply star_refl. }
+  { simpl; repeat step; eexists; split; asimpl; eapply star_trans; eauto with sred; eapply star_refl. }
+  { simpl; repeat step; eexists; split; asimpl; eapply star_trans; eauto with sred; eapply star_refl. }
+  { simpl; repeat step; eexists; split; asimpl; eapply star_trans; eauto with sred; eapply star_refl. }
+  { simpl; repeat step; eexists; split; asimpl; eapply star_trans; eauto with sred; eapply star_refl. }
+  { simpl.
+    eapply star_step_left. { eapply star_sred_fold_args; eauto. }
+    eapply star_step_right. { eapply star_sred_fold_args; eauto. }
+    eapply diagram_finish.
+  }
+  { simpl.
+    eapply star_step_left. { eapply star_sred_fold; eauto. }
+    eapply star_step_right. { eapply star_sred_fold; eauto. }
+    eapply diagram_finish.
+  }
+  { simpl.
+    eapply star_step_left. {
+      rewrite List.map_app.
+      rewrite List.map_cons.
+      rewrite map_trans_comm_value.
+      eapply star_sred_array_ctx; eauto.
+    }
+    eapply star_step_right. {
+      rewrite List.map_app.
+      rewrite List.map_cons.
+      rewrite map_trans_comm_value.
+      eapply star_sred_array_ctx; eauto.
+    }
+    eapply diagram_finish.
+  }
+  { simpl.
+    eapply step_left. {
+      rewrite List.map_app.
+      rewrite List.map_cons.
+      rewrite map_trans_comm_value.
+      simpl.
+      eapply sred_array_conflict; eauto.
+    }
+    eapply diagram_finish.
+  }
+  { simpl.
+    eapply step_left. {
+      rewrite map_trans_comm_value.
+      econstructor.
+    }
+    eapply diagram_finish.
+  }
+Admitted.
