theories/trans_definition.v
@@ -1,0 +1,254 @@
+Require Import syntax.
+Require Import small_step tactics.
+Require Import sequences.
+Require Import typing.
+
+Definition process_exceptions := 
+  (Lam (* x => *) (Lam (* y => *) 
+    (Match_ (Var 0 (* y *)) (* with *)
+      (* | None => *)
+        (Var 1 (* y *))
+      (* | Some z => *)
+        (Match_ (Var 2 (* x *)) (* with *)
+          (* | None => *)
+            (Var 1 (* y *))
+          (* | Some w => *)
+            (Conflict)
+        )
+      ))).
+
+
+Fixpoint trans_ty (ty: type): type :=
+  match ty with
+  | TBool => TBool
+  | TInteger => TInteger
+  | TFun T1 T2 => TFun (trans_ty T1) (trans_ty T2)
+  | TOption T => TOption (trans_ty T)
+  | TUnit => TUnit
+  | TDefault T => TOption (trans_ty T)
+  | TArray T => TArray (trans_ty T)
+  end
+.
+
+Fixpoint trans (t: term) : term :=
+  match t with
+  | Var x => Var x
+  | App t1 t2 => App (trans t1) (trans t2)
+  | Lam t => Lam (trans t)
+
+  | Value v => Value (trans_value v)
+  | Binop op t1 t2 => Binop op (trans t1) (trans t2)
+
+  | Match_ u t1 t2 =>
+    Match_ (trans u) (trans t1) (trans t2)
+  | ENone => ENone
+  | ESome t => ESome (trans t)
+
+  | If t ta tb =>
+    If (trans t) (trans ta) (trans tb)
+  | Fold f ts acc =>
+    Fold (trans f) (trans ts) (trans acc)
+
+  | ErrorOnEmpty t => Match_ (trans t) Conflict (Var 0)
+  | DefaultPure t => ESome (trans t)
+  | Default ts tj tc =>
+    Match_
+      (Fold 
+        process_exceptions
+        (EArray (List.map trans ts)) ENone)
+      (If (trans tj) (trans tc) ENone)
+      (ESome (Var 0))
+  | Empty => ENone
+  | Conflict => Conflict
+  | EArray ts => EArray (List.map trans ts)
+  end
+
+with trans_value v :=
+  match v with
+  | Bool b => Bool b
+  | Int i => Int i
+  | Closure t sigma => Closure (trans t) (List.map trans_value sigma)
+  | VNone => VNone
+  | VUnit => VUnit
+  | VSome v => VSome (trans_value v)
+  | VPure v => VSome (trans_value v)
+  | VArray vs => VArray (List.map trans_value vs)
+  end
+.
+
+Inductive no_default: term -> Prop :=
+  | NDVar: forall x, no_default (Var x)
+  | NDApp: forall t1 t2,
+    no_default t1 ->
+    no_default t2 ->
+    no_default (App t1 t2)
+  | NDLam: forall t,
+    no_default t ->
+    no_default (Lam t)
+
+  | NDConflict:
+    no_default Conflict
+
+  | NDValue: forall v,
+    no_default_value v ->
+    no_default (Value v)
+  | NDBinop: forall op t1 t2,
+    no_default t1 ->
+    no_default t2 ->
+    no_default (Binop op t1 t2)
+
+  | NDMatch_: forall u t1 t2,
+    no_default u ->
+    no_default t1 ->
+    no_default t2 ->
+    no_default (Match_ u t1 t2)
+  | NDENone:
+    no_default ENone
+  | NDESome: forall t,
+    no_default t ->
+    no_default (ESome t)
+  | NDFold: forall f ts t,
+    no_default f ->
+    no_default ts ->
+    no_default t ->
+    no_default (Fold f ts t)
+  | NDIf: forall t ta tb,
+    no_default t ->
+    no_default ta ->
+    no_default tb ->
+    no_default (If t ta tb)
+
+  | NDArray: forall ts,
+    List.Forall no_default ts ->
+    no_default (EArray ts)
+
+with no_default_value: value -> Prop :=
+  | NDBool: forall b, no_default_value (Bool b)
+  | NDInt: forall i, no_default_value (Int i)
+  | NDClosure: forall t sigma,
+    no_default t ->
+    List.Forall no_default_value sigma ->
+    no_default_value (Closure t sigma)
+  | NDVNone:
+    no_default_value VNone
+  | NDVUnit:
+    no_default_value VUnit
+  | NDVSome: forall v,
+    no_default_value v ->
+    no_default_value (VSome v)
+  | NDVPure: forall v,
+    no_default_value v ->
+    no_default_value (VPure v)
+  | NDVArray: forall vs,
+    List.Forall no_default_value vs ->
+    no_default_value (VArray vs)
+.
+
+
+
+Theorem no_more_defaults:
+  forall t, no_default (trans t)
+with no_more_defaults_value:
+  forall v, no_default_value (trans_value v).
+Proof.
+{ induction t; simpl; repeat econstructor; eauto.
+  { induction ts; econstructor; eauto. }
+  { induction ts; econstructor; eauto. }
+}
+{ induction v; simpl; repeat econstructor; eauto.
+  { induction sigma; econstructor; eauto. }
+  { induction ts; econstructor; eauto. }
+}
+Qed.
+
+
+Lemma trans_ty_inv_base {T}:
+  inv_base (trans_ty T)
+with trans_ty_inv_no_immediate_default {T}:
+  inv_no_immediate_default (trans_ty T).
+Proof.
+  all: induction T; simpl; econstructor; eauto.
+Qed.
+
+Lemma trans_ty_correct_term:
+  forall {t Delta Gamma T},
+    jt_term Delta Gamma t T ->
+    jt_term Delta (List.map trans_ty Gamma) (trans t) (trans_ty T)
+.
+Proof.
+  intros.
+  apply (
+    jt_term_ind'
+      (fun Delta Gamma t T => jt_term Delta (List.map trans_ty Gamma) (trans t) (trans_ty T))
+      (fun Delta t T => jt_value Delta (trans_value t) (trans_ty T))).
+
+  (* TODO: remove the timeout to put something else. *)
+  all: try solve [timeout 3 (intros; simpl; repeat econs_jt; simpl in *; eauto; repeat econs_inv; eauto using trans_ty_inv_base, trans_ty_inv_no_immediate_default)].
+  { intros; simpl; econstructor.
+    { erewrite List.map_nth_error; eauto. }
+    { eapply trans_ty_inv_base. }
+  }
+  { intros; simpl; repeat econs_jt; simpl in *; eauto using trans_ty_inv_base, trans_ty_inv_no_immediate_default.
+    12:{ clear -f2'. induction f2'; simpl; econstructor; eauto. }
+
+    all: try solve [repeat econs_inv; eauto using trans_ty_inv_base, trans_ty_inv_no_immediate_default].
+  }
+  { intros; simpl; repeat econs_jt; simpl in *; eauto using trans_ty_inv_base, trans_ty_inv_no_immediate_default. 
+    { induction op; simpl in *; inj; eauto. }
+  }
+  { intros; simpl; repeat econs_jt; simpl in *; eauto using trans_ty_inv_base, trans_ty_inv_no_immediate_default.
+    { clear -f8'; induction f8'; simpl; econstructor; eauto. }
+  }
+  { intros; simpl. eapply (JTValueClosure _ _ _ (List.map trans_ty Gamma_cl)); repeat econs_jt; simpl in *; repeat econs_inv; eauto using trans_ty_inv_base, trans_ty_inv_no_immediate_default.
+    { clear - f17'; induction f17'; econstructor; simpl; eauto. }
+    {  repeat sinv_jt; eauto. }
+  }
+  { intros; simpl; repeat econs_jt; simpl in *; eauto using trans_ty_inv_base, trans_ty_inv_no_immediate_default.
+    { clear -f22'; induction f22'; simpl; econstructor; eauto. }
+  }
+Qed.
+
+Lemma trans_ty_correct_value:
+  forall {v Delta T},
+    jt_value Delta v T ->
+    jt_value Delta (trans_value v) (trans_ty T).
+Proof.
+  intros.
+  apply (
+    jt_value_ind'
+      (fun Delta Gamma t T => jt_term Delta (List.map trans_ty Gamma) (trans t) (trans_ty T))
+      (fun Delta t T => jt_value Delta (trans_value t) (trans_ty T))).
+
+  (* TODO: remove the timeout to put something else. *)
+  all: try solve [timeout 3 (intros; simpl; repeat econs_jt; simpl in *; eauto; repeat econs_inv; eauto using trans_ty_inv_base, trans_ty_inv_no_immediate_default)].
+  { intros; simpl; econstructor.
+    { erewrite List.map_nth_error; eauto. }
+    { eapply trans_ty_inv_base. }
+  }
+  { intros; simpl; repeat econs_jt; simpl in *; eauto using trans_ty_inv_base, trans_ty_inv_no_immediate_default.
+    12:{ clear -f2'. induction f2'; simpl; econstructor; eauto. }
+
+    all: try solve [repeat econs_inv; eauto using trans_ty_inv_base, trans_ty_inv_no_immediate_default].
+  }
+  { intros; simpl; repeat econs_jt; simpl in *; eauto using trans_ty_inv_base, trans_ty_inv_no_immediate_default. 
+    { induction op; simpl in *; inj; eauto. }
+  }
+  { intros; simpl; repeat econs_jt; simpl in *; eauto using trans_ty_inv_base, trans_ty_inv_no_immediate_default.
+    { clear -f8'; induction f8'; simpl; econstructor; eauto. }
+  }
+  { intros; simpl. eapply (JTValueClosure _ _ _ (List.map trans_ty Gamma_cl)); repeat econs_jt; simpl in *; repeat econs_inv; eauto using trans_ty_inv_base, trans_ty_inv_no_immediate_default.
+    { clear - f17'; induction f17'; econstructor; simpl; eauto. }
+    {  repeat sinv_jt; eauto. }
+  }
+  { intros; simpl; repeat econs_jt; simpl in *; eauto using trans_ty_inv_base, trans_ty_inv_no_immediate_default.
+    { clear -f22'; induction f22'; simpl; econstructor; eauto. }
+  }
+Qed.
+
+Lemma trans_value_op_correct:
+  forall v op v1 v2,
+    Some v = get_op op v1 v2 ->
+    Some (trans_value v) = get_op op (trans_value v1) (trans_value v2).
+Proof.
+  induction op, v1 , v2; intros; simpl in *; inj; simpl; eauto.
+Qed.
